



The capacitance matrix is given by

$$\mathbf{C} = \begin{pmatrix} C_Q + C_g & -C_g \\ -C_g & C_r + C_g \end{pmatrix}.$$

The inverse is

$$\begin{aligned} \mathbf{C}^{-1} &= \frac{1}{(C_Q + C_g)(C_r + C_g) - C_g^2} \begin{pmatrix} C_r + C_g & C_g \\ C_g & C_Q + C_g \end{pmatrix} \\ &= \frac{1}{C_Q C_r + C_Q C_g + C_r C_g} \begin{pmatrix} C_r + C_g & C_g \\ C_g & C_Q + C_g \end{pmatrix}. \end{aligned}$$

The Hamiltonian is

$$\begin{aligned} H &= \frac{1}{2} \mathbf{q}^T \mathbf{C}^{-1} \mathbf{q} + U(\Phi) \\ &= \frac{1}{2} \frac{1}{C_Q C_r + C_Q C_g + C_r C_g} \begin{pmatrix} q_Q & q_r \end{pmatrix} \begin{pmatrix} C_r + C_g & C_g \\ C_g & C_Q + C_g \end{pmatrix} \begin{pmatrix} q_Q \\ q_r \end{pmatrix} + \frac{\Phi_r}{2L} - E_J \cos\left(\frac{2\pi}{\Phi_0} \Phi_Q\right) \\ &= \frac{1}{2} \frac{1}{C_Q C_r + C_Q C_g + C_r C_g} \left[(C_r + C_g) q_Q^2 + (C_Q + C_g) q_r^2 + 2C_g q_Q q_r \right] + \frac{\Phi_r}{2L} - E_J \cos\left(\frac{2\pi}{\Phi_0} \Phi_Q\right). \end{aligned}$$

Separating this into the three Hamiltonian terms, we get

$$\begin{aligned} H_{\text{transmon}} &= \frac{1}{2} \frac{C_r + C_g}{C_Q C_r + C_Q C_g + C_r C_g} q_Q^2 - E_J \cos\left(\frac{2\pi}{\Phi_0} \Phi_Q\right) \\ H_{\text{resonator}} &= \frac{1}{2} \frac{C_Q + C_g}{C_Q C_r + C_Q C_g + C_r C_g} q_r^2 + \frac{\Phi_r^2}{2L} \\ H_{\text{int}} &= \frac{C_g}{C_Q C_r + C_Q C_g + C_r C_g} q_Q q_r. \end{aligned}$$

We can now define the dimensionless charge number and flux operators

$$n = \frac{q}{2e}, \quad \varphi = \frac{2\pi}{\Phi_0} \Phi = \frac{\Phi}{\varphi_0},$$

to get

$$\begin{aligned} H_{\text{transmon}} &= \frac{1}{2} \frac{C_r + C_g}{\det \mathbf{C}} 4e^2 n_Q^2 - E_J \cos(\varphi_Q) \\ &= \frac{4e^2}{2\widetilde{C}_Q} n_Q^2 - E_J \cos(\varphi_Q) \\ H_{\text{resonator}} &= \frac{1}{2} \frac{C_Q + C_g}{\det \mathbf{C}} 4e^2 n_r^2 + \frac{\varphi_0^2}{2L} \varphi_r^2 \\ &= \frac{4e^2}{2\widetilde{C}_r} n_r^2 + \frac{\varphi^2}{2L} \varphi_r^2 \\ H_{\text{int}} &= \frac{C_g}{\det \mathbf{C}} 4e^2 n_Q n_r, \end{aligned}$$

where we have used the fact that the denominator is the determinant of the capacitance matrix

$$\det \mathbf{C} = (C_Q + C_g)(C_r + C_g) - C_g^2 = C_Q C_r + C_Q C_g + C_r C_g$$

and we have defined the capacitances

$$\tilde{C}_Q = \frac{\det \mathbf{C}}{C_r + C_g}, \quad \tilde{C}_r = \frac{\det \mathbf{C}}{C_Q + C_g}.$$

We now define

$$E_C = \frac{e^2}{2\tilde{C}}, \quad E_L = \frac{\varphi_0^2}{L}$$

to get

$$H_{\text{transmon}} = 4E_{C,Q}n_Q^2 - E_J \cos(\varphi_Q), \quad H_{\text{resonator}} = 4E_{C,r}n_r^2 + \frac{E_L}{2}\varphi_r^2.$$

We now quantize the Hamiltonian by promoting n and φ to operators and then writing them in terms of mode operators as

$$\hat{\varphi}_Q = \left(\frac{2E_{C,Q}}{E_J} \right)^{1/4} (\hat{b}^\dagger + \hat{b}), \quad \hat{n}_Q = \frac{i}{2} \left(\frac{E_J}{2E_{C,Q}} \right)^{1/4} (\hat{b}^\dagger - \hat{b})$$

for the transmon and

$$\hat{\varphi}_r = \left(\frac{2E_{C,r}}{E_L} \right)^{1/4} (\hat{a}^\dagger + \hat{a}), \quad \hat{n}_r = \frac{i}{2} \left(\frac{E_L}{2E_{C,r}} \right)^{1/4} (\hat{a}^\dagger - \hat{a}).$$

We see that these satisfy the commutation relations as needed

$$\begin{aligned} [\hat{\varphi}_Q, \hat{n}_Q] &= \frac{i}{2} \left(\frac{2E_{C,Q}}{E_J} \right)^{1/4} \left(\frac{E_J}{2E_{C,Q}} \right)^{1/4} [\hat{b}^\dagger + \hat{b}, \hat{b}^\dagger - \hat{b}] \\ &= \frac{i}{2} \cdot 2 \\ &= i, \\ [\hat{\varphi}_r, \hat{n}_r] &= \frac{i}{2} \left(\frac{2E_{C,r}}{E_L} \right)^{1/4} \left(\frac{E_L}{2E_{C,r}} \right)^{1/4} [\hat{a}^\dagger + \hat{a}, \hat{a}^\dagger - \hat{a}] \\ &= \frac{i}{2} \cdot 2 \\ &= i. \end{aligned}$$

The resonator Hamiltonian can be written as

$$\begin{aligned} \hat{H}_{\text{resonator}} &= 4E_{C,r} \frac{i^2}{4} \left(\frac{E_L}{2E_{C,r}} \right)^{1/2} (\hat{a}^\dagger - \hat{a})^2 + \frac{E_L}{2} \left(\frac{2E_{C,r}}{E_L} \right)^{1/2} (\hat{a}^\dagger + \hat{a})^2 \\ &= - \left(\frac{E_L E_{C,r}}{2} \right)^{1/2} (\hat{a}^\dagger \hat{a}^\dagger + \hat{a} \hat{a} - \hat{a}^\dagger \hat{a} - \hat{a} \hat{a}^\dagger) \\ &\quad + \left(\frac{E_L E_{C,r}}{2} \right)^{1/2} (\hat{a}^\dagger \hat{a}^\dagger + \hat{a} \hat{a} + \hat{a}^\dagger \hat{a} + \hat{a} \hat{a}^\dagger) \\ &= \left(\frac{E_L E_{C,r}}{2} \right)^{1/2} \cdot 2 (\hat{a}^\dagger \hat{a} + \hat{a} \hat{a}^\dagger) \\ &= \sqrt{2E_L E_{C,r}} \cdot 2 \left(\hat{a}^\dagger \hat{a} + \frac{1}{2} \right) \\ &= \sqrt{8E_L E_{C,r}} \left(\hat{a}^\dagger \hat{a} + \frac{1}{2} \right) \\ &= \hbar \omega_r \left(\hat{a}^\dagger \hat{a} + \frac{1}{2} \right), \quad \left\{ \omega_r = \frac{1}{\hbar} \sqrt{8E_L E_{C,r}} \right\} \end{aligned}$$

The interaction Hamiltonian then becomes

$$\begin{aligned} \hat{H}_{\text{int}} &= \frac{4e^2 C_g}{\det \mathbf{C}} \cdot \frac{i}{2} \left(\frac{E_J}{2E_{C,Q}} \right)^{1/4} (\hat{b}^\dagger - \hat{b}) \cdot \frac{i}{2} \left(\frac{E_L}{2E_{C,r}} \right)^{1/4} (\hat{a}^\dagger - \hat{a}) \\ &= - \frac{e^2 C_g}{\det \mathbf{C}} \left(\frac{E_J E_L}{4E_{C,Q} E_{C,r}} \right)^{1/4} (\hat{b}^\dagger - \hat{b}) (\hat{a}^\dagger - \hat{a}). \end{aligned}$$

Writing this as $\hat{H}_{\text{int}} = g(\hat{a}^\dagger - \hat{a})(\hat{b}^\dagger - \hat{b})$, where the order of \hat{a} and \hat{b} have been switched since they commute with each other, we get

$$\begin{aligned}
g &= -\frac{e^2 C_g}{\det \mathbf{C}} \left(\frac{E_J E_L}{4E_{C,Q} E_{C,r}} \right)^{1/4} \\
&= -\frac{e^2 C_g}{\det \mathbf{C}} \left(\frac{2E_L}{E_{C,r}} \right)^{1/4} \left(\frac{E_J}{8E_{C,Q}} \right)^{1/4} \\
&= -\frac{e^2 C_g}{\det \mathbf{C}} \sqrt{\frac{1}{2E_{C,r}} (8E_L E_{C,r})^{1/2}} \left(\frac{E_J}{8E_{C,Q}} \right)^{1/4} \\
&= -\frac{e^2 C_g}{\det \mathbf{C}} \sqrt{\frac{\hbar \omega_r}{2E_{C,r}}} \left(\frac{E_J}{8E_{C,Q}} \right)^{1/4} \\
&= -\frac{e^2 C_g}{\det \mathbf{C}} \sqrt{\frac{\tilde{C}_r}{e^2}} \sqrt{\hbar \omega_r} \left(\frac{E_J}{8E_{C,Q}} \right)^{1/4} \\
&= -\frac{e C_g}{\det \mathbf{C}} \sqrt{\frac{\det \mathbf{C}}{C_Q + C_g}} \sqrt{\hbar \omega_r} \left(\frac{E_J}{8E_{C,Q}} \right)^{1/4} \\
&= \boxed{-\frac{C_g}{\sqrt{C_Q + C_g}} \sqrt{\frac{\hbar \omega_r e^2}{\det \mathbf{C}}} \left(\frac{E_J}{8E_{C,Q}} \right)^{1/4}}.
\end{aligned}$$

To see it gives us the result

$$g = -\frac{C_g}{C_Q} \sqrt{\frac{\hbar \omega_r e^2}{C_r}} \left(\frac{E_J}{8E_{C,Q}} \right)^{1/4}$$

when $C_g \ll C_Q, C_r$, we first see that

$$\begin{aligned}
\tilde{C}_r &= \frac{\det \mathbf{C}}{C_Q + C_g} \\
&= \frac{C_Q C_r + C_Q C_g + C_r C_g}{C_Q + C_g} \\
&= \frac{C_r (C_Q + C_g) + C_Q C_g}{C_Q + C_g} \\
&= C_r + \frac{C_Q C_g + C_g^2 - C_g^2}{C_Q + C_g} \\
&= C_r + \frac{C_g (C_Q + C_g)}{C_Q + C_g} - \frac{C_g^2}{C_Q + C_g} \\
&\approx C_r + C_g \\
&\approx C_r.
\end{aligned}$$

Additionally,

$$\begin{aligned}
\frac{C_g}{\det \mathbf{C}} &= \frac{C_g}{C_Q C_r + C_Q C_g + C_r C_g} \\
&= \frac{C_g}{(C_Q + C_g)(C_r + C_g) - C_g^2} \\
&\approx \frac{C_g}{(C_Q + C_g)(C_r + C_g)} \\
&\approx \frac{C_g}{C_Q C_r}.
\end{aligned}$$

Then,

$$g = -\frac{e^2 C_g}{\det \mathbf{C}} \sqrt{\frac{\tilde{C}_r}{e^2}} \sqrt{\hbar \omega_r} \left(\frac{E_J}{8E_{C,Q}} \right)^{1/4}$$

$$\begin{aligned}
&\approx -\frac{C_g}{C_Q C_r} \sqrt{C_r} \sqrt{\hbar \omega_r e^2} \left(\frac{E_J}{8E_{C,Q}} \right)^{1/4} \\
&= -\frac{C_g}{C_Q} \sqrt{\frac{\hbar \omega_r e^2}{C_r}} \left(\frac{E_J}{8E_{C,Q}} \right)^{1/4}.
\end{aligned}$$

If the approximation is taken much earlier in the derivation, the definition of $E_{C,Q}$ will also now include the approximated capacitance

$$E_{C,Q} = \frac{e^2}{2\tilde{C}_Q} \approx \frac{e^2}{2(C_Q + C_g)} \approx \frac{e^2}{2C_Q}.$$